HigherCategoryTheory/SingleSorted/Cells.lean
@@ -79,4 +79,17 @@ theorem cells_sc_eq_cells_tg (k : index) (obj : Type u) [SingleSortedCategory in
   ext f
   exact cell_sc_iff_cell_tg k f
 
+section Underlying
+
+lemma underlying_source_is_cell {k m : index} (f : obj) (k_lt_m : k < m) : cell m (sc k f) := by
+  exact S.sck_scj_eq_scj f k_lt_m
+
+lemma underlying_target_is_cell {k m : index} (f : obj) (k_lt_m : k < m) : cell m (tg k f) := by
+  have : tg m (tg k f) = tg k f := by
+    exact S.tgk_tgj_eq_tgj f k_lt_m
+  apply (cell_sc_iff_cell_tg m _).mpr
+  exact this
+
+end Underlying
+
 end HigherCategoryTheory
